---
title: "TD 1 - Exercice 5"
lang: fr
author: "Théo Leroy"
date: "8 octbre 2024"
format:
  live-html:
    code-background: true
    toc: true
    page-layout: full
webr:
  render-df: gt-interactive
  resources:
    - ./../data/eucalyptus.txt
  packages:
      - dplyr
      - readr
      - ggplot2
      - cowplot
fig-align: center
editor: 
  markdown: 
    wrap: 72
---

::: {.content-hidden when-format="html"}

![](/static/img/eucalyptus.jpg){fig-align="center"}

{{< include ./../_extensions/r-wasm/live/_knitr.qmd >}}

## Question 1

L'erreur quadratique moyenne vaut

$$
\textrm{EQM}\left(\widehat{\beta} \right) = \mathbb{E}\left(\left[\widehat{\beta} -\beta \right]^2\right) =  \mathbb{V}\left(\widehat{\beta} \right) + \underbrace{\left(\mathbb{E}\left(\widehat{\beta} -\beta \right)\right)^2}_{=0 \textrm{ car } \widehat{\beta} \textrm{ est sans biais}}=\mathbb{V}\left(\widehat{\beta} \right) = \sigma^2\left(X^{'}X \right)^{-1}
$$

## Question 2

Dans le cas où $x_i=i$ pour tout $i=1, \dots, n$, on a :

$$
\begin{align*}
\overline{x_n} &= \frac{1}{n}\sum\limits_{i=1}^n x_i = \frac{1}{n}\sum\limits_{i=1}^n i =\frac{1}{n}\frac{n(n+1)}{2}=\frac{n+1}{2} \\
\sum\limits_{i=1} x_i^2 &= \sum\limits_{i=1} i^2 = \frac{n(n+1)(2n+1)}{6} \\ 
\sum\limits_{i=1}^n (x_i-\overline{x_n})^2&=\sum\limits_{i=1}^n x_i^2-n\overline{x_n}^2=\frac{n(n+1)(2n+1)}{6}-\frac{n(n+1)^2}{4}=\frac{n(n-1)(n+1)}{12} 
\end{align*}
$$

Ainsi,

$$
\textrm{EQM}\left(\widehat{\beta} \right) =\sigma^2\left(X^{'}X \right)^{-1}=
\sigma^2
\begin{pmatrix}
\frac{2(2n+1)}{n(n-1)} &
-\frac{6}{n(n-1)} \\
-\frac{6}{n(n-1)} &
\frac{12}{n(n-1)(n+1)}
\end{pmatrix}
$$

Asymptotiquement, on a alors

$$
\textrm{EQM}\left(\widehat{\beta} \right)  \underset{n\ \to\ + \infty}{\sim}\sigma^2\left(X^{'}X \right)^{-1}=
\sigma^2
\begin{pmatrix}
\frac{4}{n} &
-\frac{6}{n^2} \\
-\frac{6}{n^2} &
\frac{12}{n^3}
\end{pmatrix}
$$

## Question 3

Dans le cas où $x_i=\frac{i}{n}$ pour tout $i=1, \dots, n$, on a :

$$
\begin{align*}
\overline{x_n} &= \frac{1}{n}\sum\limits_{i=1}^n x_i = \frac{1}{n}\sum\limits_{i=1}^n \frac{i}{n} =\frac{1}{n^2}\frac{n(n+1)}{2}=\frac{n+1}{2n} \\
\sum\limits_{i=1} x_i^2 &= \sum\limits_{i=1} \frac{i^2}{n^2} = \frac{(n+1)(2n+1)}{6n} \\ 
\sum\limits_{i=1}^n (x_i-\overline{x_n})^2&=\sum\limits_{i=1}^n x_i^2-n\overline{x_n}^2=\frac{(n+1)(2n+1)}{6n}-\frac{(n+1)^2}{4n}=\frac{(n-1)(n+1)}{12n} 
\end{align*}
$$

Ainsi,

$$
\textrm{EQM}\left(\widehat{\beta} \right) =\sigma^2\left(X^{'}X \right)^{-1}=
\sigma^2
\begin{pmatrix}
\frac{2(2n+1)}{n(n-1)} &
-\frac{6}{n-1} \\
-\frac{6}{n-1} &
\frac{12n}{(n-1)(n+1)}
\end{pmatrix}
$$

Asymptotiquement, on a alors

$$
\textrm{EQM}\left(\widehat{\beta} \right)  \underset{n\ \to\ + \infty}{\sim}\sigma^2\left(X^{'}X \right)^{-1}=
\sigma^2
\begin{pmatrix}
\frac{4}{n} &
-\frac{6}{n} \\
-\frac{6}{n} &
\frac{12}{n}
\end{pmatrix}
$$

## Question 4

Dans le cas où $x_i=\frac{1}{i}$ pour tout $i=1, \dots, n$, on a :

$$
\begin{align*}
\overline{x_n} &= \frac{1}{n}\sum\limits_{i=1}^n x_i = \frac{1}{n}\sum\limits_{i=1}^n \frac{1}{i}  \\
\sum\limits_{i=1} x_i^2 &= \sum\limits_{i=1} \frac{1}{i^2} \\
\sum\limits_{i=1}^n (x_i-\overline{x_n})^2&=\sum\limits_{i=1}^n x_i^2-n\overline{x_n}^2=\frac{(n+1)(2n+1)}{6n}-\frac{(n+1)^2}{4n}=\frac{(n-1)(n+1)}{12n} 
\end{align*}
$$


:::